PaperResults.thy
@@ -2,11 +2,29 @@ theory PaperResults
   imports Loops SyntacticAssertions Compositionality TotalLogic ExamplesCompositionality
 begin
 
-text \<open>This file contains the results mentioned the paper.\<close>
+text \<open>This file contains the results mentioned the paper. It is organized in the same order and with
+the same structure as the paper. You can use the panel "Sidekick" on the right to see and navigate
+the structure of the file, via sections and subsections.
+You can ctrl+click on terms to jump to their definition.\<close>
 
-subsection \<open>Section 3\<close>
+section \<open>3: Hyper Hoare Logic\<close>
 
-subsubsection \<open>Section 3.2\<close>
+subsection \<open>3.1: Language and Semantics\<close>
+
+text \<open>The programming language is defined in the file Language.thy:
+- The type of program state is \<^typ>\<open>('pvar, 'pval) pstate\<close> (<-- you can ctrl+click on the name pstate to jump to its definition).
+- Program commands are defined as the type \<^typ>\<open>('var, 'val) stmt\<close>.
+- The big-step semantics is defined as \<^const>\<open>single_sem\<close>. We also use the notation \<^term>\<open>\<langle>C, \<sigma>\<rangle> \<rightarrow> \<sigma>'\<close>.\<close>
+
+subsection \<open>3.2: Hyper-Triples, Formally\<close>
+
+text \<open>
+- Extended states (definition 2) are defined as \<^typ>\<open>('lvar, 'lval, 'pvar, 'pval) state\<close>.
+- Hyper-assertions (definition 3) are defined in the file Logic.thy as \<^typ>\<open>('lvar, 'lval, 'pvar, 'pval) state hyperassertion\<close>.
+- The extended semantics (definition 4) is defined in the file Language.thy as \<^const>\<open>sem\<close>.
+- Lemma 1 is shown and proven below.
+- Hyper-triples (definition 5) are defined in the file Logic.thy as \<^const>\<open>hyper_hoare_triple\<close>. We
+  also use the notation \<^term>\<open>\<Turnstile> {P} C {Q}\<close>.\<close>
 
 lemma lemma1:
   "sem C (S1 \<union> S2) = sem C S1 \<union> sem C S2"
@@ -18,25 +36,36 @@ lemma lemma1:
   "sem (While C) S = (\<Union>n. iterate_sem n C S)"
   using sem_if sem_seq sem_union sem_skip sem_union_general sem_monotonic sem_while by metis+
 
-subsubsection \<open>Section 3.4\<close>
+subsection \<open>3.3: Core Rules\<close>
+
+text \<open>The core rules are defined in the file Logic.thy, as \<^const>\<open>syntactic_HHT\<close>. We also use the
+notation \<^term>\<open>\<turnstile> {P} C {Q}\<close>. Operators \<otimes> (definition 6) and \<Otimes> (definition 7) are defined as
+\<^const>\<open>join\<close> and \<^const>\<open>natural_partition\<close>, respectively.\<close>
+
+subsection \<open>3.4: Soundness and Completeness\<close>
 
 theorem thm1_soundness:
-  assumes "\<turnstile> {A} C {B}"
-  shows "\<Turnstile> {A} C {B}"
+  assumes "\<turnstile> {P} C {Q}"
+  shows "\<Turnstile> {P} C {Q}"
   using assms soundness by auto
 
 theorem thm2_completeness:
-  assumes "\<Turnstile> {A} C {B}"
-  shows "\<turnstile> {A} C {B}"
+  assumes "\<Turnstile> {P} C {Q}"
+  shows "\<turnstile> {P} C {Q}"
   using assms completeness by auto
 
-subsubsection \<open>Section 3.5\<close>
+subsection \<open>3.5: Expressivity of Hyper-Triples\<close>
 
-theorem expressing_hyperproperties_as_hyper_triples:
+text \<open>Program hyperproperties (definition 8) are defined in the file ProgramHyperproperties as
+\<^typ>\<open>('pvar, 'pval) program_hyperproperty\<close>, and the satisfiability of program hyperproperties is
+defined via the function \<^const>\<open>hypersat\<close>.\<close>
+
+theorem thm3_expressing_hyperproperties_as_hyper_triples:
   fixes to_lvar :: "'pvar \<Rightarrow> 'lvar"
   fixes to_lval :: "'pval \<Rightarrow> 'lval"
-  assumes "injective to_lvar"
-      and "injective to_lval"
+  fixes H :: "('pvar, 'pval) program_hyperproperty"
+  assumes "injective to_lvar" \<comment>\<open>The cardinality of 'lvar is at least the cardinality of 'pvar.\<close>
+      and "injective to_lval" \<comment>\<open>The cardinality of 'lval is at least the cardinality of 'pval.\<close>
     shows "\<exists>P Q::('lvar, 'lval, 'pvar, 'pval) state hyperassertion. (\<forall>C. hypersat C H \<longleftrightarrow> \<Turnstile> {P} C {Q})"
   using assms proving_hyperproperties
   by blast
@@ -47,13 +76,22 @@ theorem thm4_disproving_triples:
 
 
 
+section \<open>4: Syntactic Rules\<close>
 
+subsection \<open>4.1: Syntactic Hyper-Assertions\<close>
 
+text \<open>Syntactic hyper-expressions and hyper-assertions (definition 9) are defined in the file
+SyntacticAssertions.thy as \<^typ>\<open>'val exp\<close> and \<^typ>\<open>'val assertion\<close> respectively, where 'val is the
+type of both logical and program values. Note that we use de Bruijn indices (i.e, natural numbers)
+for quantified states and variables.\<close>
 
+subsection \<open>4.2: Syntactic Rules for Deterministic and Non-Deterministic Assignments.\<close>
 
-subsection \<open>Section 4\<close>
-
-subsubsection \<open>Section 4.2\<close>
+text \<open>We prove semantic versions of the syntactic rules from section 4 (figure 4).
+We use \<^const>\<open>interp_assert\<close> to convert a syntactic hyper-assertion into a semantic one, because
+our hyper-triples require semantic hyper-assertions. Similarly, we use \<^const>\<open>interp_pexp\<close> to convert
+a syntactic program expression into a semantic one.
+\<^term>\<open>transform_assign x pe P\<close> and \<^term>\<open>transform_havoc x P\<close> correspond to A^e_x and H_x from definition 10.\<close>
 
 proposition AssignS:
   "\<Turnstile> { interp_assert (transform_assign x pe P) } Assign x (interp_pexp pe) {interp_assert P}"
@@ -63,13 +101,24 @@ proposition HavocS:
   "\<Turnstile> { interp_assert (transform_havoc x P) } Havoc x {interp_assert P}"
   using rule_havoc_syntactic by auto
 
-subsubsection \<open>Section 4.3\<close>
+subsection \<open>4.3: Syntactic Rules for Assume Statements\<close>
+
+text \<open>\<^const>\<open>transform_assume\<close> corresponds to \<Pi>_p (definition 11). As before, we use \<^const>\<open>interp_pbexp\<close>
+to convert a syntactic program boolean expression into a semantic one.
+Similarly, \<^term>\<open>pbexp_to_assertion 0 pb\<close> converts the syntactic program boolean expression pb into
+a syntactic hyper-assertion, which applies to the state 0 (recall that we use de Bruijn indices,
+and thus state "0" corresponds to the closest quantified state.\<close>
 
 proposition AssumeS:
   "\<Turnstile> { interp_assert (transform_assume (pbexp_to_assertion 0 pb) P) } Assume (interp_pbexp pb) {interp_assert P}"
   using rule_assume_syntactic by auto
 
-subsection \<open>Section 5\<close>
+section \<open>5: Proof Principles for Loops\<close>
+
+text \<open>We show in the following our proof rules for loops, presented in figure 6. These use the following constructs:
+- \<^term>\<open>natural_partition I\<close> corresponds to the \<Otimes> operator from definition 7.
+- \<^term>\<open>lnot b\<close> negates b.
+- \<^term>\<open>while_cond b C\<close> is defined as \<^term>\<open>While (Assume b;; C);; Assume (lnot b)\<close>.\<close>
 
 theorem while_desugared:
   assumes "\<And>n. \<Turnstile> {I n} Assume b;; C {I (Suc n)}"
@@ -77,7 +126,15 @@ theorem while_desugared:
     shows "\<Turnstile> {I 0} while_cond b C { Q }"
   by (metis assms(1) assms(2) seq_rule while_cond_def while_rule)
 
-subsubsection \<open>Section 5.1\<close>
+subsection \<open>5.1: Synchronized Control Flow\<close>
+
+text \<open>In the following:
+- \<^term>\<open>conj A B\<close> corresponds to the hyper-assertion \<open>A \<and> B\<close>.
+- \<^term>\<open>holds_forall b\<close> corresponds to \<open>\<box>b\<close>.
+- \<^term>\<open>low_exp b\<close> corresponds to \<open>low(b)\<close>.
+- \<^term>\<open>disj A B\<close> corresponds to the hyper-assertion \<open>A \<or> B\<close>.
+- \<^term>\<open>emp\<close> checks whether the set of states is empty.
+- \<^term>\<open>if_then_else b C1 C2\<close> is syntactic sugar for \<^term>\<open>If (Assume b;; C1) (Assume (lnot b);; C2)\<close>.\<close>
 
 theorem WhileSync:
   assumes "\<Turnstile> {conj I (holds_forall b)} C {conj I (low_exp b)}"
@@ -91,7 +148,11 @@ theorem IfSync:
     shows "\<Turnstile> {conj P (low_exp b)} if_then_else b C1 C2 {Q}"
   using assms(1) assms(2) if_synchronized by blast
 
-subsubsection \<open>Section 5.2\<close>
+subsection \<open>5.2: \<forall>*\<exists>*-Hyperproperties\<close>
+
+text \<open>In the following:
+- \<^term>\<open>if_then b C\<close> is syntactic sugar for \<^term>\<open>If (Assume b;; C) (Assume (lnot b))\<close>.
+- \<^term>\<open>no_forall_state_after_existential Q\<close> holds iff there is no universal state quantifier \<forall>\<langle>_\<rangle> after any \<exists> in Q.\<close>
 
 theorem while_forall_exists:
   assumes "\<Turnstile> {I} if_then b C {I}"
@@ -101,7 +162,10 @@ theorem while_forall_exists:
   using while_general_syntactic[of "\<lambda>n. I"] assms
   by blast
 
-subsubsection \<open>Section 5.3\<close>
+subsection \<open>5.3: \<exists>*\<forall>*-Hyperproperties\<close>
+
+text \<open>\<^term>\<open>wfP lt\<close> in the following rule ensures that the binary operator \<open>lt\<close> is well-founded.
+\<open>e\<close> is a function of a program state, which must decrease after each iteration.\<close>
 
 theorem while_loop_exists:
   assumes "wfP lt"
@@ -112,42 +176,68 @@ theorem while_loop_exists:
 
 
 
+section \<open>Appendix A: Technical Definitions Omitted from the Paper\<close>
 
-subsection \<open>Appendix C: Expressing Judgments of Hoare Logics as Hyper-Triples\<close>
+text \<open>The following definitions are formalized in the file SyntacticAssertions.thy:
+- Evaluation of hyper-expressions (definition 12): \<^const>\<open>interp_exp\<close>.
+- Satisfiability of hyper-assertions (definition 12): \<^const>\<open>sat_assertion\<close>.
+- Syntactic transformation for deterministic assignments (definition 13): \<^const>\<open>transform_assign\<close>.
+- Syntactic transformation for non-deterministic assignments (definition 14): \<^const>\<open>transform_havoc\<close>.
+- Syntactic transformation for assume statements. (definition 15): \<^const>\<open>transform_assume\<close>.\<close>
 
-theorem prop_HL_expresses_hyperproperties:
+
+section \<open>Appendix C: Expressing Judgments of Hoare Logics as Hyper-Triples\<close>
+
+subsection \<open>Appendix C.1: Overapproximate Hoare Logics\<close>
+
+text \<open>The following judgments are defined in the file Expressivity.thy as follows:
+- Definition 16 (Hoare Logic): \<^term>\<open>HL P C Q\<close>.
+- Definition 17 (Cartesian Hoare Logic): \<^term>\<open>CHL P C Q\<close>.\<close>
+
+proposition prop_1_HL_expresses_hyperproperties:
   "\<exists>H. (\<forall>C. hypersat C H \<longleftrightarrow> HL P C Q) \<and> k_hypersafety 1 H"
   using HL_expresses_hyperproperties by blast
 
-theorem encoding_HL_in_HHL:
+proposition prop_2_expressing_HL_in_HHL:
   "HL P C Q \<longleftrightarrow> (hyper_hoare_triple (over_approx P) C (over_approx Q))"
   using encoding_HL by auto
 
-theorem encoding_CHL_in_HHL:
+proposition prop_3_CHL_is_hyperproperty:
+  "hypersat C (CHL_hyperprop P Q) \<longleftrightarrow> CHL P C Q"
+  using CHL_hyperproperty by fast
+
+proposition prop_4_encoding_CHL_in_HHL:
   assumes "not_free_var_of P x"
       and "not_free_var_of Q x"
       and "injective from_nat"
     shows "CHL P C Q \<longleftrightarrow> \<Turnstile> {encode_CHL from_nat x P} C {encode_CHL from_nat x Q}"
   using encoding_CHL assms by fast
 
-theorem CHL_is_hyperproperty:
-  "hypersat C (CHL_hyperprop P Q) \<longleftrightarrow> CHL P C Q"
-  using CHL_hyperproperty by fast
 
-lemma IL_hyperproperties:
+
+subsection \<open>Appendix C.2: Underapproximate Hoare Logics\<close>
+
+text \<open>The following judgments are defined in the file Expressivity.thy as follows:
+- Definition 18 (Incorrectness Logic): \<^term>\<open>IL P C Q\<close>.
+- Definition 19 (k-Incorrectness Logic): \<^term>\<open>RIL P C Q\<close>.
+- Definition 20 (Forward Underapproximation): \<^term>\<open>FU P C Q\<close>.
+- Definition 21 (k-Forward Underapproximation): \<^term>\<open>RFU P C Q\<close>.\<close>
+
+text \<open>RIL is the old name of k-IL, and RFU is the old name of k-FU.\<close>
+
+proposition prop_5_IL_hyperproperties:
   "IL P C Q \<longleftrightarrow> IL_hyperprop P Q (set_of_traces C)"
   using IL_expresses_hyperproperties by fast
 
-theorem encoding_IL_in_HHL:
+proposition prop_6_expressing_IL_in_HHL:
   "IL P C Q \<longleftrightarrow> (hyper_hoare_triple (under_approx P) C (under_approx Q))"
   using encoding_IL by fast
 
-text \<open>RIL is the old name of k-IL\<close>
-theorem kIL_hyperproperties:
+proposition prop_7_kIL_hyperproperties:
   "hypersat C (RIL_hyperprop P Q) \<longleftrightarrow> RIL P C Q"
   using RIL_expresses_hyperproperties by fast
 
-theorem encoding_RIL:
+proposition prop_8_expressing_kIL_in_HHL:
   fixes x :: "'lvar"
   assumes "\<And>l l' \<sigma>. (\<lambda>i. (l i, \<sigma> i)) \<in> P \<longleftrightarrow> (\<lambda>i. (l' i, \<sigma> i)) \<in> P"  (* P does not depend on logical variables *)
       and "injective (indexify :: (('a \<Rightarrow> ('pvar \<Rightarrow> 'pval)) \<Rightarrow> 'lval))" (* |lval| \<ge> |PStates^k| *)
@@ -158,17 +248,19 @@ theorem encoding_RIL:
     shows "RIL P C Q \<longleftrightarrow> \<Turnstile> {pre_insec from_nat x c P} C {post_insec from_nat x c Q}"
   using assms(1) assms(2) assms(3) assms(4) assms(5) assms(6) by (rule encoding_RIL)
 
-theorem encoding_FU_in_HHL:
-  "FU P C Q \<longleftrightarrow> \<Turnstile> {encode_FU P} C {encode_FU Q}"
-  by (rule encoding_FU)
-
-theorem FU_hyperproperties:
+proposition FU_hyperproperties:
   "hypersat C (hyperprop_FU P Q) \<longleftrightarrow> FU P C Q"
   by (rule FU_expresses_hyperproperties)
 
-text \<open>RFU is the old name of k-FU\<close>
+proposition prop_9_expressing_FU_in_HHL:
+  "FU P C Q \<longleftrightarrow> \<Turnstile> {encode_FU P} C {encode_FU Q}"
+  by (rule encoding_FU)
 
-theorem encode_RFU_in_HHL:
+proposition prop_10_kFU_expresses_hyperproperties:
+  "hypersat C (RFU_hyperprop P Q) \<longleftrightarrow> RFU P C Q"
+  by (rule RFU_captures_hyperproperties)
+
+proposition prop_11_encode_kFU_in_HHL:
   assumes "not_free_var_of P x"
       and "not_free_var_of Q x"
       and "injective from_nat"
@@ -176,21 +268,18 @@ theorem encode_RFU_in_HHL:
   using assms
   by (rule encode_RFU)
 
+subsection \<open>Appendix C.3: Beyond Over- and Underapproximation\<close>
 
-theorem RFU_expresses_hyperproperties:
-  "hypersat C (RFU_hyperprop P Q) \<longleftrightarrow> RFU P C Q"
-  by (rule RFU_captures_hyperproperties)
+text \<open>The following judgment is defined in the file Expressivity.thy as follows:
+- Definition 22 (k-Universal Existential): \<^term>\<open>RUE P C Q\<close>.
+Note that RUE is the old name of k-UE.\<close>
 
-
-
-text \<open>RUE is the old name of k-UE\<close>
-
-theorem RUE_expresses_hyperproperty:
+proposition prop_12_kUE_expresses_hyperproperty:
   "RUE P C Q \<longleftrightarrow> hypersat C (hyperprop_RUE P Q)"
   by (rule RUE_express_hyperproperties)
 
 
-theorem encoding_RUE_in_HHL:
+proposition prop_13_expressing_kUE_in_HHL:
   assumes "injective fn \<and> injective fn1 \<and> injective fn2"
       and "t \<noteq> x"
       and "injective (fn :: nat \<Rightarrow> 'a)"
@@ -198,15 +287,12 @@ theorem encoding_RUE_in_HHL:
       and "injective fn2"
       and "not_in_free_vars_double {x, t} P"
       and "not_in_free_vars_double {x, t} Q"
-
   shows "RUE P C Q \<longleftrightarrow> \<Turnstile> {encode_RUE_1 fn fn1 fn2 x t P} C {encode_RUE_2 fn fn1 fn2 x t Q}"
   using assms by (rule encoding_RUE)
 
 
-
-
-text \<open>Example 4\<close>
-theorem proving_refinement:
+text \<open>Example 3\<close>
+proposition proving_refinement:
   fixes P :: "(('lvar \<Rightarrow> 'lval) \<times> ('pvar \<Rightarrow> 'pval)) set \<Rightarrow> bool"
   assumes "(a :: 'pval) \<noteq> b"
     (* and x free var *)
@@ -227,49 +313,51 @@ theorem proving_refinement:
 
 
 
-subsection \<open>Appendix D: Compositionality\<close>
+section \<open>Appendix D: Compositionality\<close>
 
-subsubsection \<open>Rules from D.1\<close>
+subsection \<open>Appendix D.1: Compositionality Rules\<close>
 
-proposition Linking:
+text \<open>In the following, we show the rules from figure 11, in the order in which they appear.\<close>
+
+proposition rule_Linking:
   assumes "\<And>\<phi>1 (\<phi>2 :: ('a, 'b, 'c, 'd) state). fst \<phi>1 = fst \<phi>2 \<and> ( \<Turnstile> { (in_set \<phi>1 :: (('a, 'b, 'c, 'd) state) hyperassertion) } C { in_set \<phi>2 } )
   \<Longrightarrow> ( \<Turnstile> { (P \<phi>1 :: (('a, 'b, 'c, 'd) state) hyperassertion) } C { Q \<phi>2 } )"
   shows "\<Turnstile> { ((\<lambda>S. \<forall>\<phi>1 \<in> S. P \<phi>1 S) :: (('a, 'b, 'c, 'd) state) hyperassertion) } C { (\<lambda>S. \<forall>\<phi>2 \<in> S. Q \<phi>2 S) }"
   using assms by (rule rule_linking)
 
-proposition And_rule:
-  assumes "\<Turnstile> {P} C {Q}"
-      and "hyper_hoare_triple P' C Q'"
-    shows "hyper_hoare_triple (conj P P') C (conj Q Q')"
-  using assms by (rule rule_And)
-
-proposition Or_rule:
+proposition rule_And:
   assumes "\<Turnstile> {P} C {Q}"
       and "\<Turnstile> {P'} C {Q'}"
-    shows "hyper_hoare_triple (disj P P') C (disj Q Q')"
+    shows "\<Turnstile> {conj P P'} C {conj Q Q'}"
+  using assms by (rule rule_And)
+
+proposition rule_Or:
+  assumes "\<Turnstile> {P} C {Q}"
+      and "\<Turnstile> {P'} C {Q'}"
+    shows "\<Turnstile> {disj P P'} C {disj Q Q'}"
   using assms by (rule rule_Or)
 
-proposition FrameSafe:
+proposition rule_FrameSafe:
   assumes "wr C \<inter> fv F = {}"
       and "wf_assertion F"
       and "no_exists_state F"
     shows "\<Turnstile> {interp_assert F} C {interp_assert F}"
   using safe_frame_rule_syntactic assms by auto
 
-proposition Forall_rule:
+proposition rule_Forall:
   assumes "\<And>x. \<Turnstile> {P x} C {Q x}"
-  shows "hyper_hoare_triple (forall P) C (forall Q)"
+  shows "\<Turnstile> {forall P} C {forall Q}"
   using assms by (rule rule_Forall)
 
 proposition rule_IndexedUnion:
   assumes "\<And>x. \<Turnstile> {P x} C {Q x}"
-  shows "hyper_hoare_triple (general_join P) C (general_join Q)"
+  shows "\<Turnstile> {general_join P} C {general_join Q}"
   using assms by (rule rule_IndexedUnion)
 
 proposition rule_Union:
   assumes "\<Turnstile> {P} C {Q}"
-      and "hyper_hoare_triple P' C Q'"
-    shows "hyper_hoare_triple (join P P') C (join Q Q')"
+      and "\<Turnstile> {P'} C {Q'}"
+    shows "\<Turnstile> {join P P'} C {join Q Q'}"
   using assms by (rule rule_Union)
 
 proposition rule_BigUnion:
@@ -278,7 +366,7 @@ proposition rule_BigUnion:
   shows "\<Turnstile> {general_union P} C {general_union Q}"
   using assms by (rule rule_BigUnion)
 
-proposition Specialize:
+proposition rule_Specialize:
   assumes "\<Turnstile> {interp_assert P} C {interp_assert Q}"
       and "indep_of_set b"
       and "wf_assertion_aux 0 1 b"
@@ -286,14 +374,18 @@ proposition Specialize:
     shows "\<Turnstile> { interp_assert (transform_assume b P) } C { interp_assert (transform_assume b Q) }"
   using filter_rule_syntactic assms by blast
 
-proposition LUpdate:
+text \<open>In the following, \<^term>\<open>entails_with_updates vars P P'\<close> and \<^term>\<open>invariant_on_updates vars Q\<close>
+respectively correspond to the notions of entailments modulo logical variables and invariance with
+respect to logical updates, as described in definition 23.\<close>
+
+proposition rule_LUpdate:
   assumes "\<Turnstile> {P'} C {Q}"
       and "entails_with_updates vars P P'"
       and "invariant_on_updates vars Q"
     shows "\<Turnstile> {P} C {Q}"
   using assms by (rule rule_LUpdate)
 
-proposition LUpdateSyntactic:
+proposition rule_LUpdateSyntactic:
   assumes "\<Turnstile> { (\<lambda>S. P S \<and> e_recorded_in_t e t S) } C { Q }"
       and "not_fv_hyper t P"
       and "not_fv_hyper t Q"
@@ -312,24 +404,21 @@ proposition rule_AtLeast:
   using assms by (rule rule_AtLeast)
 
 proposition rule_True:
-  "hyper_hoare_triple P C (\<lambda>_. True)"
+  "\<Turnstile> {P} C {\<lambda>_. True}"
   by (rule rule_True)
 
 proposition rule_False:
-  "hyper_hoare_triple (\<lambda>_. False) C Q"
+  "\<Turnstile> { (\<lambda>_. False) } C {Q}"
   by (rule rule_False)
 
 proposition rule_Empty:
   "\<Turnstile> { (\<lambda>S. S = {}) } C { (\<lambda>S. S = {}) }"
   by (rule rule_Empty)
 
+subsection \<open>Appendix D.2: Examples\<close>
 
 
-
-subsubsection \<open>Examples from D.2\<close>
-
-
-proposition composing_monotonicity_and_minimum:
+proposition fig_12_composing_monotonicity_and_minimum:
   fixes P :: "((('a \<Rightarrow> 'b) \<times> ('c \<Rightarrow> 'd)) set \<Rightarrow> bool)"
   fixes i :: 'a
   fixes x y :: 'c
@@ -343,10 +432,7 @@ proposition composing_monotonicity_and_minimum:
     shows "\<Turnstile> { P } C1 ;; C2 { has_minimum y leq }"
   using assms by (rule composing_monotonicity_and_minimum)
 
-
-
-
-proposition composing_GNI_with_SNI:
+proposition fig_13_composing_GNI_with_SNI:
   fixes h :: 'lvar
   fixes l :: 'pvar
   assumes "\<Turnstile> { (low l :: (('lvar, 'lval, 'pvar, 'pval) state) hyperassertion) } C2 { low l }"
@@ -358,33 +444,30 @@ proposition composing_GNI_with_SNI:
 
 
 
+section \<open>Appendix E: Termination-Based Reasoning\<close>
 
+text \<open>Total hyper-triples (definition 24) are defined as \<^const>\<open>total_hyper_triple\<close>, and usually
+written \<^term>\<open>\<Turnstile>TOT {P} C {Q}\<close>.\<close>
 
-
-subsection \<open>Appendix E: Termination-Based Reasoning\<close>
-
-
-
-theorem while_synchronized_total:
-  assumes "wfP lt"
-      and "\<And>n. not_fv_hyper t (I n)"
-      and "\<And>n. \<Turnstile>TOT {conj (conj (I n) (holds_forall b)) (e_recorded_in_t e t)} C {conj (conj (I (Suc n)) (low_exp b)) (e_smaller_than_t e t lt)}"
-    shows "\<Turnstile>TOT {conj (I 0) (low_exp b)} while_cond b C {conj (exists I) (holds_forall (lnot b))}"
-  using assms while_synchronized_tot by meson
-
-theorem frame_rule:
+theorem rule_Frame:
   assumes "\<Turnstile>TOT {P} C {Q}"
       and "wr C \<inter> fv F = {}"
       and "wf_assertion F"
     shows "\<Turnstile>TOT {conj P (interp_assert F)} C {conj Q (interp_assert F)}"
   by (simp add: assms(1) assms(2) assms(3) frame_rule_syntactic)
 
+theorem rule_WhileSyncTot:
+  assumes "wfP lt"
+      and "\<And>n. not_fv_hyper t (I n)"
+      and "\<And>n. \<Turnstile>TOT {conj (conj (I n) (holds_forall b)) (e_recorded_in_t e t)} C {conj (conj (I (Suc n)) (low_exp b)) (e_smaller_than_t e t lt)}"
+    shows "\<Turnstile>TOT {conj (I 0) (low_exp b)} while_cond b C {conj (exists I) (holds_forall (lnot b))}"
+  using assms while_synchronized_tot by meson
 
 
 
-subsection \<open>Appendix I: Synchronous Reasoning over Different Branches\<close>
+section \<open>Appendix H: Synchronous Reasoning over Different Branches\<close>
 
-theorem synchronized_if_rule:
+proposition prop_14_synchronized_if_rule:
   assumes "\<Turnstile> {P} C1 {P1}"
       and "\<Turnstile> {P} C2 {P2}"
       and "\<Turnstile> {combine from_nat x P1 P2} C {combine from_nat x R1 R2}"
@@ -397,7 +480,5 @@ theorem synchronized_if_rule:
       and "not_free_var_hyper x R2"
     shows "\<Turnstile> {P} If (Seq C1 (Seq C C1')) (Seq C2 (Seq C C2')) {join Q1 Q2}"
   using if_sync_rule assms by fast
-
-
 
 end
